theories/Compositional_Structures/Basic_Modules/Component_Types/Electoral_Module_Ref.thy
@@ -5,7 +5,8 @@ theory Electoral_Module_Ref
            Refine_Imperative_HOL.IICF
 begin                            
 
-type_synonym 'a Electoral_Module_Ref = "'a set \<Rightarrow> 'a Profile_List \<Rightarrow> 'a Result"
+
+type_synonym 'a Electoral_Module_Ref = "'a set \<Rightarrow> 'a Profile_List \<Rightarrow> 'a Result nres"
 
 definition electoral_module_r :: " 'a Electoral_Module_Ref \<Rightarrow> bool" where
   "electoral_module_r mr \<equiv> \<forall> A pa. well_formed A (mr A pa)"
@@ -29,4 +30,6 @@ lemma em_onA:
   shows "(em_r A pa) = (em A (pl_to_pr_\<alpha> pa))"
   by (metis assms(1) assms(2) brI pair_in_Id_conv tagged_fun_relD_rhs)
 
+
+type_synonym 'a Electoral_Module_SepRef = "nat set \<Rightarrow> 'a Profile_List \<Rightarrow> 'a Result"
 end
